auto_generated/isabelle/Import_everything.thy
@@ -55,7 +55,7 @@ imports
 	 "/auto/homes/dpm36/Work/Cambridge/bitbucket/linksem/auto_generated/isabelle/Abi_power64_elf_header" 
 	 "/auto/homes/dpm36/Work/Cambridge/bitbucket/linksem/auto_generated/isabelle/Abi_power64_section_header_table" 
 	 "/auto/homes/dpm36/Work/Cambridge/bitbucket/linksem/auto_generated/isabelle/Abi_x86_relocation" 
-
+  "Archive"
 begin 
 
 (** [import_everything] imports all Lem files for convenience when testing the
